@prefix owl:   <http://www.w3.org/2002/07/owl#> .
@prefix gsp:   <http://www.opengis.net/ont/geosparql#> .
@prefix rdf:   <http://www.w3.org/1999/02/22-rdf-syntax-ns#> .
@prefix xsd:   <http://www.w3.org/2001/XMLSchema#> .
@prefix skos:  <http://www.w3.org/2004/02/skos/core#> .
@prefix rdfs:  <http://www.w3.org/2000/01/rdf-schema#> .
@prefix glosis: <http://w3id.org/glosis/model/glosis#> .
@prefix lcc-cr: <https://www.omg.org/spec/LCC/Countries/CountryRepresentation/> .
@prefix om:    <http://www.ontology-of-units-of-measure.org/resource/om-2/> .
@prefix foaf:  <http://xmlns.com/foaf/0.1/> .
@prefix ssn:   <http://www.w3.org/ns/ssn/> .
@prefix sosa:  <http://www.w3.org/ns/sosa/> .
### ISO FEATURES
@prefix iso19156_SF:  <http://def.isotc211.org/iso19156/2011/SamplingFeature#> .
@prefix iso19156_SSF:  <http://def.isotc211.org/iso19156/2011/SpatialSamplingFeature#> .
@prefix iso19156_GFI: 	<http://def.isotc211.org/iso19156/2011/GeneralFeatureInstance#> .
@prefix iso28258: 	<http://www.iso28258.org#> .


glosis:cropClass  a      owl:ObjectProperty ;
        rdfs:range       sosa:ObservableProperty ;
        skos:definition  "Result should be of type CropClassValue\nObservedProperty = CropClass"@en .

glosis:cropDescription
        a                owl:DatatypeProperty ;
        rdfs:range       xsd:string ;
        skos:definition  "Description of crops at the site"@en .

glosis:geology  a        owl:ObjectProperty ;
        rdfs:range       sosa:ObservableProperty ;
        skos:definition  "Result should be of type LithologyValue\nObservedProperty = Geology\nUnclear what the FoI is here"@en .

glosis:country
        a            owl:ObjectProperty ;
        rdfs:range   lcc-cr:Alpha2Code .


glosis:soilDepthRootable
        a                owl:ObjectProperty ;
        rdfs:range       sosa:Observation ;
        skos:definition  "UoM in cm\nResult of type Integer\nObservedProperty = SoilDepthRootable"@en .

glosis:slopeOrientationClass
        a                owl:ObjectProperty ;
        rdfs:range       sosa:ObservableProperty ;
        skos:definition  "Result should be of type SlopeOrientationClassValue\nObservedProperty = SlopeOrientationClass"@en .


glosis:erosionCategory
        a                owl:ObjectProperty ;
        rdfs:range       sosa:ObservableProperty ;
        skos:definition  "Result should be of type ErosionCategoryValue\nObservedProperty =  ErosionCategory"@en .

glosis:erosionAreaAffected
        a                owl:ObjectProperty ;
        rdfs:range       sosa:ObservableProperty ;
        skos:definition  "Result should be of type ErosionAreaAffectedValue\nObservedProperty = ErosionAreaAffected"@en .

glosis:landUseRemark  a  owl:DatatypeProperty ;
        rdfs:range       xsd:string ;
        skos:definition  "Description of land use at the site"@en .

glosis:landUseCropRotation
        a                owl:DatatypeProperty ;
        rdfs:range       xsd:string ;
        skos:definition  "Description of crop rotation at the site"@en .


glosis:weatheringFragments
        a                owl:ObjectProperty ;
        rdfs:range       sosa:ObservableProperty ;
        skos:definition  "Result of type WeatheringValue (Table 29)\nObservedProperty = weatheringFragments"@en .

glosis:remarks
        a            owl:DatatypeProperty ;
        rdfs:range   xsd:string .

glosis:parentTextureUnconsolidated
        a                owl:ObjectProperty ;
        rdfs:range       sosa:ObservableProperty ;
        skos:definition  "Result should be of type TextureUnconsolidatedValue\nObservedProperty = ParentTexture"@en .

glosis:landUseGrass  a   owl:ObjectProperty ;
        rdfs:range       sosa:Observation ;
        skos:definition  "Result should be an Integer\nUoM is percentage\nObservedProperty = GrassAbundance"@en .


glosis:surfaceAge  a     owl:ObjectProperty ;
        rdfs:range       sosa:ObservableProperty ;
        skos:definition  "Result should be of type SurfaceAgeValue\nObservedProperty = SurfaceAge"@en .

glosis:weatheringRock
        a                owl:ObjectProperty ;
        rdfs:range       sosa:ObservableProperty ;
        skos:definition  "Result should be of type WeatheringValue (Table 29)\nObservedProperty = weatheringRock"@en .

glosis:slopeForm  a      owl:ObjectProperty ;
        rdfs:range       sosa:ObservableProperty ;
        skos:definition  "Result should be of type SlopeFormValue\nObservedProperty = SlopeForm"@en .

glosis:altitude
        a            owl:DatatypeProperty ;
        rdfs:range   om:Measure .

glosis:slopeOrientationNumeric
        a                owl:ObjectProperty ;
        rdfs:range       sosa:Observation ;
        skos:definition  "Result expressed as an integer\nObservedProperty = SlopeOrientation"@en .

glosis:GL_Plot  a        owl:Class ;
        #rdfs:subClassOf  gsp:Feature ;
        rdfs:subClassOf  iso28258:Plot ;
        rdfs:subClassOf  [ a                owl:Restriction ;
                           owl:cardinality  "1"^^xsd:nonNegativeInteger ;
                           owl:onProperty   glosis:location
                         ] ;
        rdfs:subClassOf  [ a                owl:Restriction ;
                           owl:cardinality  "1"^^xsd:nonNegativeInteger ;
                           owl:onProperty   glosis:remarks
                         ] ;
        rdfs:subClassOf  [ a                owl:Restriction ;
                           owl:cardinality  "1"^^xsd:nonNegativeInteger ;
                           owl:onProperty   glosis:responsibleOrganization
                         ] ;
        rdfs:subClassOf  [ a                owl:Restriction ;
                           owl:cardinality  "1"^^xsd:nonNegativeInteger ;
                           owl:onProperty   glosis:positionalAccuracy
                         ] ;
        rdfs:subClassOf  [ a                owl:Restriction ;
                           owl:cardinality  "1"^^xsd:nonNegativeInteger ;
                           owl:onProperty   glosis:altitude
                         ] ;
        rdfs:subClassOf  [ a                owl:Restriction ;
                           owl:cardinality  "1"^^xsd:nonNegativeInteger ;
                           owl:onProperty   glosis:timestamp
                         ] ;
        rdfs:subClassOf  [ a                owl:Restriction ;
                           owl:cardinality  "1"^^xsd:nonNegativeInteger ;
                           owl:onProperty   glosis:mapSheetID
                         ] ;
        rdfs:subClassOf  [ a                owl:Restriction ;
                           owl:cardinality  "1"^^xsd:nonNegativeInteger ;
                           owl:onProperty   glosis:country
                         ] .

glosis:parentLithology
        a                owl:ObjectProperty ;
        rdfs:range       sosa:ObservableProperty ;
        skos:definition  "Result should be of type LithologyValue\nObservedProperty = ParentLithology\nUnclear what the FoI is here"@en .

glosis:soilDepthSampled
        a                owl:ObjectProperty ;
        rdfs:range       sosa:Observation ;
        skos:definition  "UoM in cm\nNote: this attribute may be an artifact!!!\nResult of type Integer\nObservedProperty = DepthSampled"@en .

glosis:slopeGradientClass
        a                owl:ObjectProperty ;
        rdfs:range       sosa:ObservableProperty ;
        skos:definition  "Result should be of type SlopeGradientClassValue\nObservedProperty = SlopeGradientClass"@en .


glosis:erosionDegree  a  owl:ObjectProperty ;
        rdfs:range       sosa:ObservableProperty ;
        skos:definition  "Result should be of type ErosionDegreeValue\nObservedProperty = ErosionDegree"@en .

glosis:landformComplex
        a                owl:ObjectProperty ;
        rdfs:range       sosa:ObservableProperty ;
        skos:definition  "Result should be of type LandformComplexValue\nObservedProperty = LandformComplex"@en .

glosis:landUseBareCover
        a                owl:ObjectProperty ;
        rdfs:range       sosa:Observation ;
        skos:definition  "Result should be an Integer\nUoM is percentage\nObservedProperty = BareCoverAbundance"@en .

glosis:weatherPast  a    owl:ObjectProperty ;
        rdfs:range       sosa:ObservableProperty ;
        skos:definition  "Result should be of type WeatherConditionsValue\nObservedProperty = WeatherConditionsPast"@en .

<http://w3id.org/glosis/model/glosis>
        a                owl:Ontology ;
        #owl:imports      foaf: , ssn: , lcc-cr: , <https://github.com/HajoRijgersberg/OM/raw/master/om-2.0.rdf> , sosa: , <http://www.opengis.net/ont/geosparql> ;
        owl:imports      ssn: , sosa: ;
        owl:versionIRI   "http://w3id.org/glosis/model/glosis/1.0" ;
        owl:versionInfo  "1.0" .

glosis:soilDepth  a      owl:ObjectProperty ;
        rdfs:range       sosa:Observation ;
        skos:definition  "UoM in cm\nResult of type Integer\nObservedProperty = Depth"@en .

glosis:koeppenClass  a   owl:ObjectProperty ;
        rdfs:range       sosa:ObservableProperty ;
        skos:definition  "Missing Codelist for KÃ¶ppen Classes\nResult should be of type KoeppenClassValue\nObservedProperty = KoeppenClass"@en .

glosis:rockOutcropsCover
        a                owl:ObjectProperty ;
        rdfs:range       sosa:ObservableProperty ;
        skos:definition  "Result should be of type RockOutcropsCoverValue\nObservedProperty = RockOutcropsCover"@en .

glosis:parentDeposition
        a                owl:ObjectProperty ;
        rdfs:range       sosa:ObservableProperty ;
        skos:definition  "Result should be of type ErosionCategoryValue\nObservedProperty = ParentDeposition\nUnclear what the FoI is here"@en .

glosis:physiographyDescription
        a                owl:DatatypeProperty ;
        rdfs:range       xsd:string ;
        skos:definition  "Description of the local physiography"@en .


glosis:floodDuration  a  owl:ObjectProperty ;
        rdfs:range       sosa:ObservableProperty ;
        skos:definition  "Currently references Table 174, which doesn't exist!\nResult should be of type FloodDurationValue\nObservedProperty = FloodDuration"@en .

glosis:location
        a            owl:DatatypeProperty ;
        rdfs:range   xsd:string .

glosis:physiography  a   owl:ObjectProperty ;
        rdfs:range       sosa:ObservableProperty ;
        skos:definition  "Result should be of type PhysiographyValue\nObservedProperty = Physiography"@en .

glosis:parentRemarks  a  owl:DatatypeProperty ;
        rdfs:range       xsd:string ;
        skos:definition  "Remarks on the parent material"@en .

glosis:mapSheetID
        a            owl:DatatypeProperty ;
        rdfs:range   xsd:string .

glosis:slopeGradientNumeric
        a                owl:ObjectProperty ;
        rdfs:range       sosa:Observation ;
        skos:definition  "Result expressed as a Real,\nUoM percentage value\nObservedProperty = SlopeGradient"@en .

glosis:vegetationDescription
        a                owl:DatatypeProperty ;
        rdfs:range       xsd:string ;
        skos:definition  "Description of vegetation at the site"@en .

glosis:landUseForest  a  owl:ObjectProperty ;
        rdfs:range       sosa:Observation ;
        skos:definition  "Result should be an Integer\nUoM is percentage\nObservedProperty = ForestAbundance"@en .

glosis:rockOutcropsDistance
        a                owl:ObjectProperty ;
        rdfs:range       sosa:ObservableProperty ;
        skos:definition  "Result should be of type RockOutcropsDistanceValue\nObservedProperty = RockOutcropsDistance"@en .

glosis:soilDepthRootableClass
        a                owl:ObjectProperty ;
        rdfs:range       sosa:ObservableProperty ;
        skos:definition  "Result of type SoilDepthRootableValue\nObservedProperty = SoilDepthRootableClass"@en .

glosis:landUsePavedCover
        a                owl:ObjectProperty ;
        rdfs:range       sosa:Observation ;
        skos:definition  "Result should be an Integer\nUoM is percentage\nObservedProperty = PavedAbundance"@en .

glosis:slopePathways  a  owl:ObjectProperty ;
        rdfs:range       sosa:ObservableProperty ;
        skos:definition  "Result should be of type SlopePathwaysValue\nObservedProperty = SlopePathways"@en .

glosis:majorLandform  a  owl:ObjectProperty ;
        rdfs:range       sosa:ObservableProperty ;
        skos:definition  "Result should be of type MajorLandformValue\nObservedProperty =  MajorLandform"@en .

glosis:positionalAccuracy
        a            owl:ObjectProperty ;
        rdfs:range   ssn:Property .

glosis:groundwaterDepth
        a                owl:ObjectProperty ;
        rdfs:range       sosa:Observation ;
        skos:definition  "Result should be of type Real\nObservedProperty = GroundwaterDepth"@en .

glosis:lithology  a      owl:ObjectProperty ;
        rdfs:range       sosa:ObservableProperty ;
        skos:definition  "Result should be of type LithologyValue\nObservedProperty = Lithology\nUnclear what the FoI is here"@en .

glosis:weatherCurrent
        a                owl:ObjectProperty ;
        rdfs:range       sosa:ObservableProperty ;
        skos:definition  "Result should be of type WeatherConditionsValue\nObservedProperty = WeatherConditionsCurrent"@en .

glosis:floodFrequency
        a                owl:ObjectProperty ;
        rdfs:range       sosa:ObservableProperty ;
        skos:definition  "Currently references Table 174, which doesn't exist!\nResult should be of type FloodFrequencyValue\nObservedProperty = FloodFrequency"@en .

glosis:humanInfluenceClass
        a                owl:ObjectProperty ;
        rdfs:range       sosa:ObservableProperty ;
        skos:definition  "Result should be of type HumanInfluenceClassValue\nObservedProperty = HumanInfluenceClass"@en .

glosis:soilDepthBedrock
        a                owl:ObjectProperty ;
        rdfs:range       sosa:Observation ;
        skos:definition  "ObservedProperty = DepthBedrock\nResult of type Integer"@en .

glosis:responsibleOrganization
        a            owl:ObjectProperty ;
        rdfs:range   foaf:Agent .

glosis:landUseShrubs  a  owl:ObjectProperty ;
        rdfs:range       sosa:Observation ;
        skos:definition  "Result should be an Integer\nUoM is percentage\nObservedProperty = ShrubsAbundance"@en .

glosis:timestamp
        a            owl:ObjectProperty ;
        rdfs:range   xsd:dateTime .

glosis:GL_Site  a        owl:Class ;
        #rdfs:subClassOf  gsp:Feature ;
        rdfs:subClassOf  iso28258:Site ;
        rdfs:subClassOf  [ a                owl:Restriction ;
                           owl:cardinality  "1"^^xsd:nonNegativeInteger ;
                           owl:onProperty   glosis:country
                         ] ;
        rdfs:subClassOf  [ a                owl:Restriction ;
                           owl:cardinality  "1"^^xsd:nonNegativeInteger ;
                           owl:onProperty   glosis:location
                         ] ;
        rdfs:subClassOf  [ a                owl:Restriction ;
                           owl:cardinality  "1"^^xsd:nonNegativeInteger ;
                           owl:onProperty   glosis:mapSheetID
                         ] ;
        rdfs:subClassOf  [ a                owl:Restriction ;
                           owl:cardinality  "1"^^xsd:nonNegativeInteger ;
                           owl:onProperty   glosis:positionalAccuracy
                         ] ;
        rdfs:subClassOf  [ a                owl:Restriction ;
                           owl:cardinality  "1"^^xsd:nonNegativeInteger ;
                           owl:onProperty   glosis:timestamp
                         ] ;
        rdfs:subClassOf  [ a                owl:Restriction ;
                           owl:cardinality  "1"^^xsd:nonNegativeInteger ;
                           owl:onProperty   glosis:remarks
                         ] ;
        rdfs:subClassOf  [ a                owl:Restriction ;
                           owl:cardinality  "1"^^xsd:nonNegativeInteger ;
                           owl:onProperty   glosis:altitude
                         ] ;
        rdfs:subClassOf  [ a                owl:Restriction ;
                           owl:cardinality  "1"^^xsd:nonNegativeInteger ;
                           owl:onProperty   glosis:responsibleOrganization
                         ] .

glosis:erosionActivityPeriod
        a                owl:ObjectProperty ;
        rdfs:range       sosa:ObservableProperty ;
        skos:definition  "Result should be of type ErosionActivityPeriodValue\nObservedProperty = ErosionActivityPeriod"@en .

glosis:vegetationClass
        a                owl:ObjectProperty ;
        rdfs:range       sosa:ObservableProperty ;
        skos:definition  "Result should be of type VegetationClassValue\nObservedProperty = VegetationClass"@en .

glosis:treeDensity  a    owl:ObjectProperty ;
        rdfs:range       sosa:Observation ;
        skos:definition  "result should be Boolean\nUoM in n/ha\nObservedProperty = TreeDensity"@en .

glosis:erosionTotalAreaAffected
        a                owl:ObjectProperty ;
        rdfs:range       sosa:ObservableProperty ;
        skos:definition  "Result should be of type ErosionTotalAreaAffectedValue\nObservedProperty = ErosionTotalAreaAffected"@en .

glosis:landUseClass  a   owl:ObjectProperty ;
        rdfs:range       sosa:ObservableProperty ;
        skos:definition  "Result should be of type LandUseClassValue\nObservedProperty = LandUseClass"@en .

### ISO FEATURES

iso19156_GFI:GFI_Feature
  a owl:Class ;
  rdfs:label "GFI_Feature" ;
  skos:definition """The class GFI_Feature (Figure 2) is an instance of the .og.metaclass.cg. GF_FeatureType (ISO 19109). It represents the set of all classes which are feature types. NOTE	GFI_Feature is implemented in GML (ISO 19136:2007) by the element gml:AbstractFeature and type gml:AbstractFeatureType. In an implementation this abstract class shall be substituted by a concrete class representing a feature type from an application schema associated with a domain of discourse (ISO 19109, ISO 19101). Sampling Features (Clause 8) are a class of feature-types whose role is primarily associated with observations. """ ;
  rdfs:isDefinedBy <http://standards.iso.org/iso/19156/ed-1/en/> .
  
iso19156_GFI:GFI_DomainFeature
  a owl:Class ;
  rdfs:label "GFI_DomainFeature" ;
  skos:definition "The class GFI_DomainFeature represents 'real-world' features which are the ultimate subject of an observation campaign, i.e. the features from an application domain that are .lt.i.gt.not .lt..sl.i.gt.artefacts of the observation process (sampling features). " ;
  rdfs:isDefinedBy <http://standards.iso.org/iso/19156/ed-1/en/> ;
  rdfs:subClassOf iso19156_GFI:GFI_Feature .

iso19156_SF:SF_SamplingFeature
  a owl:Class ;
  rdfs:label "SF_SamplingFeature" ;
  skos:definition ".lt.ul.gt.	.lt.li.gt..lt.b.gt.Role of sampling features.lt..sl.b.gt..lt..sl.li.gt..lt..sl.ul.gt.Sampling features are artefacts of an observational strategy, and have no significant function outside of their role in the observation process. The physical characteristics of the features themselves are of little interest, except perhaps to the manager of a sampling campaign.EXAMPLE	A .ldq.station.rdq. is essentially an identifiable locality where a sensor system or procedure may be deployed and an observation made. In the context of the observation model, it connotes the .ldq.world in the vicinity of the station.rdq., so the observed properties relate to the physical medium at the station, and not to any physical artefact such as a mooring, buoy, benchmark, monument, well, etc. NOTE	A transient sampling feature, such as a ships-track or flight-line, may be identified and described, but is unlikely to be revisited exactly. A sampling feature is intended to sample some feature of interest in an application domain. However, in some cases the identity, and even the exact type, of the sampled feature may not be known when observations are made using the sampling features. .lt.ul.gt.	.lt.li.gt..lt.b.gt.Classification of sampling features.lt..sl.b.gt..lt..sl.li.gt..lt..sl.ul.gt.A small number of sampling patterns are common across disciplines in observational science. These provide a basis for processing and portrayal tools which are similar across domains, and depend primarily on the geometry of the sample design. Common names for sampling features include specimen, station, profile, transect, path, swath, and scene. These are classified primarily by their topological dimension. Point-located samples are defined in this Clause, extensive samples of various dimensions in Clause 9 and specimens in Clause 10." ;
  rdfs:isDefinedBy <http://standards.iso.org/iso/19156/ed-1/en/> ;
  rdfs:subClassOf <http://def.isotc211.org/iso19156/2011/GeneralFeatureInstance#GFI_Feature> .
  
iso19156_SSF:SF_SpatialSamplingFeature
  a owl:Class ;
  rdfs:label "SF_SpatialSamplingFeature" ;
  skos:definition "When observations are made to estimate properties of a geospatial feature, in particular where the value of a property varies within the scope of the feature, a spatial sampling feature is used. Depending on accessibility and on the nature of the expected property variation, the sampling feature may be extensive in one, two or three spatial dimensions. Processing and visualization methods are often dependent on the topological dimension of the sampling manifold, so this provides a natural classification system for sampling features.  This classification follows common practice in focussing on conventional spatial dimensions. Properties observed on sampling features may be time-dependent, but the temporal axis does not generally contribute to the classification of sampling feature classes. Sampling feature identity is usually less time-dependent than is the property value." ;
  rdfs:isDefinedBy <http://standards.iso.org/iso/19156/ed-1/en/> ;
  rdfs:subClassOf <http://def.isotc211.org/iso19156/2011/SamplingFeature#SF_SamplingFeature> .    

iso19156_SF:SF_SamplingFeature.sampledFeature 
  a owl:ObjectProperty ;
  rdfs:label "sampledFeature" ;
  rdfs:isDefinedBy <http://standards.iso.org/iso/19156/ed-1/en/> ;
  rdfs:domain iso19156_SF:SF_SamplingFeature ;
  rdfs:range iso19156_GFI:GFI_DomainFeature, iso19156_GFI:GFI_Feature .  
  
iso28258:Plot  
	a owl:Class ;
  rdfs:label "Plot" ;
  skos:definition "elementary area where individual observations are made and/or samples are taken" ;
  rdfs:isDefinedBy <https://www.iso.org/obp/ui/#iso:std:iso:28258:ed-1:v1:en> ;
  rdfs:subClassOf iso19156_SSF:SF_SpatialSamplingFeature .  
  
iso28258:Site  
	a owl:Class ;
  rdfs:label "Site" ;
  skos:definition "defined area which is subject to a soil quality investigation" ;
  rdfs:isDefinedBy <https://www.iso.org/obp/ui/#iso:std:iso:28258:ed-1:v1:en> .
  
#################################################################
#    Alignments
#################################################################

gsp:Feature owl:equivalentClass iso19156_GFI:GFI_Feature .
sosa:FeatureOfInterest rdfs:subClassOf iso19156_GFI:GFI_DomainFeature .
sosa:Sample owl:equivalentClass iso19156_SF:SF_SamplingFeature .
sosa:isSampleOf owl:equivalentProperty iso19156_SF:SF_SamplingFeature.sampledFeature .